CookLevin/Complexity/NP/GenNP.lean
@@ -5,10 +5,13 @@ set_option autoImplicit false
 structure GenNPInput (X__cert : Type) [encodable X__cert] where
   rel : X__cert → Prop
   rel_poly : inTimePoly rel
+  maxSize : Nat
+  steps : Nat
+  rel_size : ∀ ⦃cert⦄, rel cert → encodable.size cert ≤ maxSize
 
 def GenNP (X__cert : Type) [encodable X__cert] : GenNPInput X__cert → Prop :=
-  fun inst => ∃ cert : X__cert, inst.rel cert
+  fun inst => ∃ cert : X__cert, encodable.size cert ≤ inst.maxSize ∧ inst.rel cert
 
 theorem genNP_iff {X__cert : Type} [encodable X__cert] (inst : GenNPInput X__cert) :
-    GenNP X__cert inst ↔ ∃ cert : X__cert, inst.rel cert := by
+    GenNP X__cert inst ↔ ∃ cert : X__cert, encodable.size cert ≤ inst.maxSize ∧ inst.rel cert := by
   rfl
