CookLevin/Complexity/L_to_LM.lean
@@ -7,10 +7,14 @@ set_option autoImplicit false
 def genNPToLMGenNPInstance {X : Type} [encodable X] (inst : GenNPInput X) :
     LMGenNP.Instance X where
   source := inst
-  maxSize := 0
-  steps := 0
+  maxSize := inst.maxSize
+  steps := inst.steps
 
 theorem GenNP_to_LMGenNP (X : Type) [encodable X] :
     GenNP X ⪯p LMGenNP.LMGenNP X := by
   refine ⟨⟨genNPToLMGenNPInstance, by sorry, fun {inst} => ?_⟩⟩
-  sorry
+  constructor
+  · rintro ⟨cert, hsize, hrel⟩
+    exact ⟨cert, hsize, hsize, hrel⟩
+  · rintro ⟨cert, hsize, _, hrel⟩
+    exact ⟨cert, hsize, hrel⟩
